Protocol/ServiceProvider.fst
@@ -5,29 +5,34 @@ open Protocol
 - Protocol events
 - Add assumtions
 - Add asserts
+- Fork
 *)
 
-val serviceprovider: me:prin -> client:prin -> idp:prin -> unit 
-let serviceprovider me client idp = 
-  
-  let reqRes = recieve client in (*1*)
+val serviceprovider: me:prin -> client:prin -> idp:prin -> pubkey idp -> unit 
+let serviceprovider me client idp pubkidp = 
+    (* Generate keypair *)
+  let pubk, privk = keygen me in
+
+    let reqRes = recieve client in (*1*)
   match reqRes with
   | HttpGet (uri) -> 
   
-    let (authnReq, sigSP)  = CreateAuthnRequest me idp in 
-    assume(Log idp "relay") (*Protocol event*);
-  
-  	let authnReqest = SamlProtocolMessage idp authnReq sigSP "relay" in 
-  	send client authnReqest; (*2*)
-  
-  	let authResponse = recieve client in (*7*)
-  	match authResponse with
-  	| SamlProtocolMessage (sp, message, sigIDP, relay) -> 
-  
-  		let resource = Resource uri in
-  		send client resource	(*8*)
-  
-  	| _ ->  send client (Failed (403))(*8.1*)     
+    let authnReq = createAuthnRequest me idp in 
+    assume(Log me authnReq) (*Protocol event*);
+    let sigSP = sign me privk authnReq in
+      
+    let authnReqest = SamlProtocolMessage idp authnReq sigSP uri in 
+    send client authnReqest; (*2*)  
+    let authResponse = recieve client in (*7*)
+    match authResponse with
+    | SamlProtocolMessage (sp, message, sigIDP, relay) -> 
+      (if verify idp pubkidp message sigIDP
+      then
+        ((*assert(Log idp message);*)
+          let resource = Resource uri in
+          send client resource)  (*8*)
+      else ())
+    | _ ->  send client (Failed (403))(*8.1*)     
   
   | _ -> send client (Failed (400))(*2.1*)
 
