Protocol/identityprovider.fst
@@ -7,35 +7,42 @@ open Protocol
 - Add asserts
 *)
 
-val identityprovider: me:prin -> client:prin -> sp:prin -> unit
-let identityprovider me client serviceprovider =
+val identityprovider: me:prin -> client:prin -> sp:prin -> pubkey sp -> unit
+let identityprovider me client serviceprovider pubksp =
 	
+  (* Generate keypair *)
+  let pubk, privk = keygen me in
+
   let authRequest = recieve client in (*3*)
 	match authRequest with
-	| SamlProtocolMessage (idp, message, sigSP, relay)-> 
-    
-    
+	| SamlProtocolMessage (idp, message, sigSP, relay)->  
 
-    let challenge = CreateChallenge client in
-    (*assert (Log serviceprovider relay );*)
-    let challengeMessage = Challenge challenge in
-    send client challengeMessage; (*4*)
+    if verify serviceprovider pubksp message sigSP
+    then
+     ( (*assert (Log serviceprovider message);*)
+        let challenge = createChallenge client in
     
-    let credentials = recieve client in (*5*)
-      match credentials with
-      | Credentials(user, password, challenge') -> 
+        let challengeMessage = ChallengeMessage challenge in
+        send client challengeMessage; (*4*)
+        let credentials = recieve client in (*5*)
+        match credentials with
+          | Credentials(user, password, challenge') -> 
   
-        (*Check credentials and challenge*)
+          (*Check credentials and challenge*)
   
-        let (samlresponse, sigIDP) = CreateSamlResponse me serviceprovider Success in
-        let response = SamlProtocolMessage serviceprovider samlresponse sigIDP relay in
-        send client response(*6*)
+          let samlresponse = createSamlResponse me serviceprovider Success in
+          assume(Log me samlresponse);
+          let sigIDP = sign me privk samlresponse in 
+          let response = SamlProtocolMessage serviceprovider samlresponse sigIDP relay in
+          send client response(*6*)
   
-      | _ -> send client (Failed (400))(*6.3*)
-	
+        | _ -> send client (Failed (400)))(*6.3*)
+    else send client (Failed (400))
   | _ -> 
-    let (samlresponse, sigIDP) = CreateSamlResponse me serviceprovider Requester in
-    let response = SamlProtocolMessage serviceprovider samlresponse sigIDP relay in
-    send client response (*4.1*)
+     let samlresponse = createSamlResponse me serviceprovider Requester in
+     assume(Log me samlresponse);
+     let sigIDP = sign me privk samlresponse in
+     let response = SamlProtocolMessage serviceprovider samlresponse sigIDP "" in
+     send client response (*4.1*)
 
 end (*Identityprovider*)
