Protocol/main.fst
@@ -5,6 +5,7 @@ open Client
 
 val main: sp:prin -> res:uri -> user:string -> password:string -> unit
 let main sp resource user password = 
+	print_string "Entering Main";
 	let req = HttpGet resource in
 		let message = client sp req user password in
 		()
