build.ps1
@@ -1,2 +1,0 @@
-mkdir -p bin
-fstar --genIL --writePrims --odir bin --dotnet4 --parallel simplesaml.fst
